---
author:
  name: "Yoseobmite"
date: 2020-07-11
title: GS Macro
categories:
- newBlog
tag: 
- markdown
- hugo
- myblog
thumbnailImagePosition: left
thumbnailImage: //live.staticflickr.com/65535/50100129036_a6142b9400_b.jpg
#autoThumbnailImage: yes
coverImage: //www.ghibli.jp/images/buta1.jpg
coverSize : partial
metaAlignment: center
showDate: true
showTags: true
showPagination: true
showSocial: true
showMeta: true
showActions: true
---

### gist 
{{< gist yoseobmite fd3d384b5edb8f4437a3d71e660b473b >}}

### image 

Goldman Sachs Macro At a Glance


{{< image src="https://user-images.githubusercontent.com/33090364/87234211-27b45e00-c3cf-11ea-858a-67c12c22a259.png" alt="GS Macro" position="center" max-width="80%" height="auto" >}} 


### latex  

```
$$\int_{a}^{b} x^2 dx$$
```

The following

$$\int_{a}^{b} x^2 dx$$

Is an integral

```
$$
\begin{align}
\vec{a} \cdot \vec{b} &= |\vec{a}||\vec{b}|cos\theta \\\\\
&= a_1b_1+a_2b_2
\end{align}
$$
```
$$
\begin{align}
\vec{a} \cdot \vec{b} &= |\vec{a}||\vec{b}|cos\theta \\\\\
&= a_1b_1+a_2b_2
\end{align}
$$

```
$$
\begin{align}
A^{\[0\]} & = Input Feature & (1) \\\\\
Z^{\[1\]} & = W^{\[1\]}A^{\[0\]} & (2) \\\\\
A^{\[1\]} & = g(Z^{\[1\]}) & (3) \\\\\
Z^{\[2\]} & = W^{\[2\]}A^{\[1\]} & (4) \\\\\
A^{\[2\]} & = g(Z^{\[2\]}) & (5)
\end{align}
$$
```

$$
\begin{align}
A^{\[0\]} & = Input Feature & (1) \\\\\
Z^{\[1\]} & = W^{\[1\]}A^{\[0\]} & (2) \\\\\
A^{\[1\]} & = g(Z^{\[1\]}) & (3) \\\\\
Z^{\[2\]} & = W^{\[2\]}A^{\[1\]} & (4) \\\\\
A^{\[2\]} & = g(Z^{\[2\]}) & (5)
\end{align}
$$

```
$$
\begin{align}
Cost & = \frac{1}{2}(\hat{Y}-Y)^2  & (1)\\\\\
\frac{\partial Cost}{\partial A^{\[2\]}} & = \hat{Y}-Y & (2)\\\\\  
sigmoid(Z^{\[l\]]}) & = sigmoid(Z^{\[l\]]})(1-sigmoid(Z^{\[l\]]})) & (3)\\\\\
& = A^{\[l\]}(1-A^{\[l\]}) \\\\\
\frac{\partial Z^{\[l\]}}{\partial W^{\[2\]}} & = \frac{\partial A^{\[l-1\]}W^{\[l\]}}{\partial W^{\[l\]}} = A^{\[l-1\]} & (4) \\\\\  
\end{align}
$$
```
$$
\begin{align}
Cost & = \frac{1}{2}(\hat{Y}-Y)^2  & (1)\\\\\
\frac{\partial Cost}{\partial A^{\[2\]}} & = \hat{Y}-Y & (2)\\\\\  
sigmoid(Z^{\[l\]]}) & = sigmoid(Z^{\[l\]]})(1-sigmoid(Z^{\[l\]]})) & (3)\\\\\
& = A^{\[l\]}(1-A^{\[l\]}) \\\\\
\frac{\partial Z^{\[l\]}}{\partial W^{\[2\]}} & = \frac{\partial A^{\[l-1\]}W^{\[l\]}}{\partial W^{\[l\]}} = A^{\[l-1\]} & (4) \\\\\  
\end{align}
$$


```
$$
\begin{align}
\Delta W^{\[2\]} & = \frac{\partial Cost}{\partial W^{\[2\]}} \\\\\
& = \frac{\partial Cost}{\partial A^{\[2\]}}\frac{\partial A^{\[2\]}}{\partial W^{\[2\]}} \\\\\
& =  \frac{\partial Cost}{\partial A^{\[2\]}}\frac{\partial A^{\[2\]}}{\partial Z^{\[2\]}}\frac{\partial Z^{\[2\]}}{\partial W^{\[2\]}} \\\\\
& =  (\hat{y}-y)\frac{\partial A^{\[2\]}}{\partial Z^{\[2\]}}\frac{\partial Z^{\[2\]}}{\partial W^{\[2\]}} \\\\\
& =  (\hat{y}-y)g'(z^{\[2\]})\frac{\partial Z^{\[2\]}}{\partial W^{\[2\]}} \\\\\
& =  (\hat{y}-y)sigmoid'(z^{\[2\]})\frac{\partial Z^{\[2\]}}{\partial W^{\[2\]}} \\\\\
& =  (\hat{y}-y)A^{\[2\]}(1-A^{\[2\]})\frac{\partial Z^{\[2\]}}{\partial W^{\[2\]}} \\\\\
& =  (\hat{y}-y)A^{\[2\]}(1-A^{\[2\]})A^{\[1\]}
\end{align}
$$
```

$$
\begin{align}
\Delta W^{\[2\]} & = \frac{\partial Cost}{\partial W^{\[2\]}} \\\\\
& = \frac{\partial Cost}{\partial A^{\[2\]}}\frac{\partial A^{\[2\]}}{\partial W^{\[2\]}} \\\\\
& =  \frac{\partial Cost}{\partial A^{\[2\]}}\frac{\partial A^{\[2\]}}{\partial Z^{\[2\]}}\frac{\partial Z^{\[2\]}}{\partial W^{\[2\]}} \\\\\
& =  (\hat{y}-y)\frac{\partial A^{\[2\]}}{\partial Z^{\[2\]}}\frac{\partial Z^{\[2\]}}{\partial W^{\[2\]}} \\\\\
& =  (\hat{y}-y)g'(z^{\[2\]})\frac{\partial Z^{\[2\]}}{\partial W^{\[2\]}} \\\\\
& =  (\hat{y}-y)sigmoid'(z^{\[2\]})\frac{\partial Z^{\[2\]}}{\partial W^{\[2\]}} \\\\\
& =  (\hat{y}-y)A^{\[2\]}(1-A^{\[2\]})\frac{\partial Z^{\[2\]}}{\partial W^{\[2\]}} \\\\\
& =  (\hat{y}-y)A^{\[2\]}(1-A^{\[2\]})A^{\[1\]}
\end{align}
$$

```
$$
\begin{align}
\Delta W^{\[2\]} & =
  \begin{bmatrix}
    \Delta w^{\[1\]}11 & \Delta w^{\[1\]}12   \\\\\
  \end{bmatrix} \\\\\
  & =\begin{bmatrix}
    (\hat{y}-y)a^{\[2\]}_1(1-a^{\[2\]}_1)a^{\[1\]}_1 & (\hat{y}-y)a^{\[2\]}_1(1-a^{\[2\]}_1)a^{\[1\]}_2   \\\\\
  \end{bmatrix} \\\\\
  & =(\hat{y}-y)a^{\[2\]}_1(1-a^{\[2\]}_1) \begin{bmatrix}
    a^{\[1\]}_1 & a^{\[1\]}_2   \\\\\
  \end{bmatrix}
\end{align}
$$
```

$$
\begin{align}
\Delta W^{\[2\]} & =
  \begin{bmatrix}
    \Delta w^{\[1\]}11 & \Delta w^{\[1\]}12   \\\\\
  \end{bmatrix} \\\\\
  & =\begin{bmatrix}
    (\hat{y}-y)a^{\[2\]}_1(1-a^{\[2\]}_1)a^{\[1\]}_1 & (\hat{y}-y)a^{\[2\]}_1(1-a^{\[2\]}_1)a^{\[1\]}_2   \\\\\
  \end{bmatrix} \\\\\
  & =(\hat{y}-y)a^{\[2\]}_1(1-a^{\[2\]}_1) \begin{bmatrix}
    a^{\[1\]}_1 & a^{\[1\]}_2   \\\\\
  \end{bmatrix}
\end{align}
$$

```
$$
\begin{align}
OutputRowSize & = \frac{InputRowSize}{PoolingSize} \\\\\
OutputColumnSize & = \frac{InputColumnSize}{PoolingSize}
\end{align}
$$
```

$$
\begin{align}
OutputRowSize & = \frac{InputRowSize}{PoolingSize} \\\\\
OutputColumnSize & = \frac{InputColumnSize}{PoolingSize}
\end{align}
$$

```
$$
\begin{align}
Row Size & = \frac{36}{2} = 18 \\\\\
Column Size & =  \frac{28}{2} = 14  
\end{align}
$$
```

$$
\begin{align}
Row Size & = \frac{36}{2} = 18 \\\\\
Column Size & =  \frac{28}{2} = 14  
\end{align}
$$

```
$$
\begin{align}
Row Size & = \frac{N-F}{Strid} + 1 = \frac{18-3}{1} + 1 = 16 \\\\\
Column Size & =  \frac{N-F}{Strid} + 1 = \frac{14-3}{1} + 1 = 12  
\end{align}
$$
```

$$
\begin{align}
Row Size & = \frac{N-F}{Strid} + 1 = \frac{18-3}{1} + 1 = 16 \\\\\
Column Size & =  \frac{N-F}{Strid} + 1 = \frac{14-3}{1} + 1 = 12  
\end{align}
$$

```
$$
cost(W, b) = \frac{1}{m}\sum_i^m{L(\hat{y^i}, y^i)} + \lambda\frac{1}{2}||w||^2
$$
</font>
```

$$
cost(W, b) = \frac{1}{m}\sum_i^m{L(\hat{y^i}, y^i)} + \lambda\frac{1}{2}||w||^2
$$
</font>

```
$$
L_p = (\sum_i^n |x_i|^p)^{\frac{1}{p}}
$$
</font>
```

$$
L_p = (\sum_i^n |x_i|^p)^{\frac{1}{p}}
$$
</font>

```
$$
\begin{align}
L_1 & = (\sum_i^n |x_i|) \\\\\
& = |x_1| + |x_2| + |x_3| + .... + |x_n|  
\end{align}
$$
```

$$
\begin{align}
L_1 & = (\sum_i^n |x_i|) \\\\\
& = |x_1| + |x_2| + |x_3| + .... + |x_n|  
\end{align}
$$

```
$$
\begin{align}
x & = [1, 2, 3, 4, 5] \\\\\
||x||_1 & = (|1| +|2| +|3| +|4| +|5|) \\\\\
& = 15
\end{align}
$$
```

$$
\begin{align}
x & = [1, 2, 3, 4, 5] \\\\\
||x||_1 & = (|1| +|2| +|3| +|4| +|5|) \\\\\
& = 15
\end{align}
$$

```
>$$
\begin{align}
tanh(x) & = \frac{1-e^{-x}}{1+e^{-x}} \\\\\
& = \frac{2}{1+e^{-2x}} -1
\end{align}
$$
```

>$$
\begin{align}
tanh(x) & = \frac{1-e^{-x}}{1+e^{-x}} \\\\\
& = \frac{2}{1+e^{-2x}} -1
\end{align}
$$

```
>$$
\begin{align}
sigmoid(x) & = \frac{1}{1+e^{-x}}  \\\\\
tanh(x) & = 2sigmoid(2x) -1
\end{align}
$$
```

>$$
\begin{align}
sigmoid(x) & = \frac{1}{1+e^{-x}}  \\\\\
tanh(x) & = 2sigmoid(2x) -1
\end{align}
$$

```
$$
\begin{align}
(e^{x})' &= e^{x} \\\\\
(e^{-x})' &= -e^{-x} \\\\\
\big[ \frac{f(x)}{g(x)}\big]' & = \frac{f'(x)g(x)-f(x)g'(x)}{g^2(x)}
\end{align}
$$
```

$$
\begin{align}
(e^{x})' &= e^{x} \\\\\
(e^{-x})' &= -e^{-x} \\\\\
\big[ \frac{f(x)}{g(x)}\big]' & = \frac{f'(x)g(x)-f(x)g'(x)}{g^2(x)}
\end{align}
$$

```
>$$
\begin{align}
f(x) & = e^{x}-e^{-x} \\\\\
g(x) & = e^{x}+e^{-x} \\\\\
\frac{d}{dx}tanh(x) & = \big[\frac{e^{x}-e^{-x}}{e^{x}+e^{-x}}\big]' \\\\\
 & =  \big[\frac{f(x)}{g(x)}\big]' \\\\\
 & = \frac{f'(x)g(x)-f(x)g'(x)}{g^2(x)} \\\\\
 & = \frac{(e^{x}-(-e^{-x}))(e^{x}+e^{-x}) - (e^{x}-e^{-x})(e^{x}-e^{-x} )}{(1+e^{-x})^2} \\\\\
 & = \frac{(e^{x}+e^{-x})^2 - (e^{x}-e^{-x})^2}{(e^{x}+e^{-x})^2} \\\\\
 & = \frac{(e^{x}+e^{-x})^2}{(e^{x}+e^{-x})^2} - \frac{(e^{x}-e^{-x})^2}{(e^{x}+e^{-x})^2} \\\\\
 & = 1 - \big[\frac{(e^{x}-e^{-x})}{(e^{x}+e^{-x})}\big]^2 \\\\\
 & = 1 - tanh^2(x) \\\\\
 & = (1 - tanh(x))(1 + tanh(x))
\end{align}
$$
```

>$$
\begin{align}
f(x) & = e^{x}-e^{-x} \\\\\
g(x) & = e^{x}+e^{-x} \\\\\
\frac{d}{dx}tanh(x) & = \big[\frac{e^{x}-e^{-x}}{e^{x}+e^{-x}}\big]' \\\\\
 & =  \big[\frac{f(x)}{g(x)}\big]' \\\\\
 & = \frac{f'(x)g(x)-f(x)g'(x)}{g^2(x)} \\\\\
 & = \frac{(e^{x}-(-e^{-x}))(e^{x}+e^{-x}) - (e^{x}-e^{-x})(e^{x}-e^{-x} )}{(1+e^{-x})^2} \\\\\
 & = \frac{(e^{x}+e^{-x})^2 - (e^{x}-e^{-x})^2}{(e^{x}+e^{-x})^2} \\\\\
 & = \frac{(e^{x}+e^{-x})^2}{(e^{x}+e^{-x})^2} - \frac{(e^{x}-e^{-x})^2}{(e^{x}+e^{-x})^2} \\\\\
 & = 1 - \big[\frac{(e^{x}-e^{-x})}{(e^{x}+e^{-x})}\big]^2 \\\\\
 & = 1 - tanh^2(x) \\\\\
 & = (1 - tanh(x))(1 + tanh(x))
\end{align}
$$

```
>$$
\begin{align}
\frac{d}{dx}tanh(x) & = 1- tanh^2(x) \\\\\
 & = (1-tanh(x))(1+tanh(x)) \\\\\
\end{align}
$$
```

>$$
\begin{align}
\frac{d}{dx}tanh(x) & = 1- tanh^2(x) \\\\\
 & = (1-tanh(x))(1+tanh(x)) \\\\\
\end{align}
$$


